refactored up until revocation

theories/ftlr/interp_weakening.v
@@ -6,12 +6,13 @@ From cap_machine Require Import ftlr_base monotone region.
 From cap_machine Require Import addr_reg.
 
 Section fundamental.
-  Context `{memG Σ, regG Σ, STSG Σ, logrel_na_invs Σ,
-            MonRef: MonRefG (leibnizO _) CapR_rtc Σ,
-            Heap: heapG Σ}.
+  Context {Σ:gFunctors} {memg:memG Σ} {regg:regG Σ}
+          {stsg : STSG Addr region_type Σ} {heapg : heapG Σ}
+          `{MonRef: MonRefG (leibnizO _) CapR_rtc Σ} {nainv: logrel_na_invs Σ}.
 
   Notation STS := (leibnizO (STS_states * STS_rels)).
-  Notation WORLD := (leibnizO (STS * STS)). 
+  Notation STS_STD := (leibnizO (STS_std_states Addr region_type)).
+  Notation WORLD := (prodO STS_STD STS). 
   Implicit Types W : WORLD.
 
   Notation D := (WORLD -n> (leibnizO Word) -n> iProp Σ).
@@ -26,7 +27,7 @@ Section fundamental.
                (∃ p', ⌜PermFlows p p'⌝ ∗
                 ([∗ list] a ∈ (region_addrs b e),
                  (read_write_cond a p' interp) ∧
-                 ⌜if pwl p then region_state_pwl W a else region_state_nwl W a l⌝ ∧ ⌜region_std W a⌝) ∗
+                 ⌜if pwl p then region_state_pwl W a else region_state_nwl W a l⌝) ∗
                 (□ match p with RX | RWX | RWLX => exec_cond W b e l p interp | _ => True end) ∗
                 (⌜if pwl p then l = Local else True⌝)))%I).
   Proof.
@@ -45,7 +46,7 @@ Section fundamental.
   Qed.
 
   Definition IH: iProp Σ :=
-    (□ ▷ (∀ (a7 : leibnizO (STS * STS)) (a8 : Reg) (a9 : Perm) (a10 : Locality) 
+    (□ ▷ (∀ (a7 : WORLD) (a8 : Reg) (a9 : Perm) (a10 : Locality) 
            (a11 a12 a13 : Addr),
             full_map a8
                      -∗ (∀ r1 : RegName,
@@ -57,7 +58,7 @@ Section fundamental.
                                 end)
                      -∗ registers_mapsto (<[PC:=inr (a9, a10, a11, a12, a13)]> a8)
                      -∗ region a7
-                     -∗ sts_full_world sts_std a7
+                     -∗ sts_full_world a7
                      -∗ na_own logrel_nais ⊤
                      -∗ ⌜a9 = RX ∨ a9 = RWX ∨ a9 = RWLX ∧ a10 = Local⌝
             → □ (∃ p'0 : Perm,
@@ -66,8 +67,7 @@ Section fundamental.
                        read_write_cond a14 p'0 interp
                        ∧ ⌜if pwl a9
                           then region_state_pwl a7 a14
-                          else region_state_nwl a7 a14 a10⌝
-                               ∧ ⌜region_std a7 a14⌝)) -∗ 
+                          else region_state_nwl a7 a14 a10⌝)) -∗ 
                 interp_conf a7))%I.
 
   (* TODO: move to region.v *)
@@ -80,35 +80,22 @@ Section fundamental.
     reflexivity.
   Qed.
 
-  (* TODO: Move somewhere *)
-  Lemma region_std_future W W' l x:
-    (@future_world Σ l W W' -∗
-    ⌜region_std W x⌝ -∗
-    ⌜region_std W' x⌝)%I.
-  Proof.
-    iIntros "A B"; rewrite !/region_std.
-    destruct l; simpl; iDestruct "A" as "%"; iDestruct "B" as "%".
-    - iPureIntro; eapply related_sts_rel_std; eauto.
-    - iPureIntro; eapply rel_is_std_i_monotone; eauto.
-  Qed.
-
   (* TODO: Move in monotone ? *)
   Lemma region_state_nwl_future W W' l l' p a:
     LocalityFlowsTo l' l ->
     (if pwl p then l = Local else True) ->
     (@future_world Σ l' W W') -∗
-    ⌜region_std W a⌝ -∗
     ⌜if pwl p then region_state_pwl W a else region_state_nwl W a l⌝ -∗
     ⌜region_state_nwl W' a l'⌝.
   Proof.
-    intros Hlflows Hloc. iIntros "Hfuture % %".
+    intros Hlflows Hloc. iIntros "Hfuture %".
     destruct l'; simpl; iDestruct "Hfuture" as "%"; iPureIntro.
     - assert (l = Global) as -> by (destruct l; simpl in Hlflows; tauto).
       destruct (pwl p); try congruence.
       eapply region_state_nwl_monotone_nl; eauto.
     - destruct (pwl p).
       + subst l. left. eapply region_state_pwl_monotone; eauto.
-      + generalize (region_state_nwl_monotone _ _ _ _ a0 H3 a1).
+      + generalize (region_state_nwl_monotone _ _ _ _ H a0).
         destruct l; auto.
   Qed.
 
@@ -117,15 +104,14 @@ Section fundamental.
     LocalityFlowsTo l' l ->
     (if pwl p then l = Local else True) ->
     (@future_world Σ l' W W') -∗
-    ⌜region_std W a⌝ -∗
     ⌜if pwl p then region_state_pwl W a else region_state_nwl W a l⌝ -∗
     ⌜if pwl p' then region_state_pwl W' a else region_state_nwl W' a l'⌝.
   Proof.
-    intros Hpflows Hlflows Hloc. iIntros "Hfuture % %".
+    intros Hpflows Hlflows Hloc. iIntros "Hfuture %".
     case_eq (pwl p'); intros.
     - assert (pwl p = true) as Hpwl.
-      { destruct p, p'; simpl in H3; try congruence; simpl in Hpflows; try tauto. }
-      rewrite Hpwl in a1, Hloc. subst l.
+      { destruct p, p'; simpl in H; try congruence; simpl in Hpflows; try tauto. }
+      rewrite Hpwl in a0, Hloc. subst l.
       destruct l'; simpl in Hlflows; try tauto.
       simpl; iDestruct "Hfuture" as "%"; iPureIntro.
       eapply region_state_pwl_monotone; eauto.
@@ -138,20 +124,6 @@ Section fundamental.
   Proof.
     rewrite /PermFlows; split; intros; auto.
     destruct (Is_true_reflect (PermFlowsTo p p')); auto.
-  Qed.
-
-  (* TODO: move to sts.v ?*)
-  Lemma related_sts_pub_world_refl W:
-    related_sts_pub_world W W.
-  Proof.
-    split; eapply related_sts_pub_refl.
-  Qed.
-
-  (* TODO: move to sts.v ?*)
-  Lemma related_sts_priv_world_refl W:
-    related_sts_priv_world W W.
-  Proof.
-    split; eapply related_sts_priv_refl.
   Qed.
 
   Lemma interp_weakening W p p' l l' b b' e e' a a':
@@ -184,25 +156,24 @@ Section fundamental.
       iExists p''; iSplitR; eauto. destruct (Addr_le_dec b' e').
       - rewrite (isWithin_region_addrs_decomposition b' e' b e); try solve_addr.
         rewrite !big_sepL_app. iDestruct "A" as "[A1 [A2 A3]]".
-        iApply (big_sepL_impl with "A2"); auto. iAlways; iIntros (k x Hx) "[#X [% %]]".
+        iApply (big_sepL_impl with "A2"); auto. iAlways; iIntros (k x Hx) "[#X %]".
         repeat iSplitR; auto.
-        + iApply (region_state_nwl_future with "Hfuture"); eauto.
-        + iApply (region_std_future with "Hfuture"); eauto.
+        iApply (region_state_nwl_future with "Hfuture"); eauto.
       - rewrite (region_addrs_empty b' e'); auto. solve_addr. }
     assert (Hpfl: PermFlows p' p'') by (eapply PermFlows_trans; eauto; eapply PermFlowsToPermFlows; eauto).
     iExists p''; iSplitR; auto. iSplit.
     { destruct (Addr_le_dec b' e').
       - rewrite (isWithin_region_addrs_decomposition b' e' b e); try solve_addr.
         rewrite !big_sepL_app. iDestruct "A" as "[A1 [A2 A3]]".
-        iApply (big_sepL_impl with "A2"); auto. iAlways; iIntros (k x Hx) "[#X [% %]]".
+        iApply (big_sepL_impl with "A2"); auto. iAlways; iIntros (k x Hx) "[#X %]".
         repeat iSplit; auto.
         case_eq (pwl p'); intros.
         + assert (pwl p = true) as HP by (destruct p, p'; simpl in Hp; inv Hp; simpl in *; auto; try congruence).
-          rewrite HP in H5. iPureIntro. auto.
+          rewrite HP in H1. iPureIntro. auto.
         + iApply region_state_nwl_future; eauto.
           destruct l'; iPureIntro.
-          * eapply related_sts_priv_world_refl.
-          * eapply related_sts_pub_world_refl.
+          * eapply related_sts_priv_refl_world.
+          * eapply related_sts_pub_refl_world.
       - rewrite (region_addrs_empty b' e'); auto. solve_addr. }
     iSplit.
     { iModIntro. assert ((p' = RX \/ p' = RWX \/ p' = RWLX) \/ (p' <> RX /\ p' <> RWX /\ p' <> RWLX)) as Hp'.
@@ -221,21 +192,20 @@ Section fundamental.
           - destruct Hp' as [-> | [-> | ->] ]; auto. iPureIntro; right; right.
             split; auto.
             destruct l'; auto. destruct p; simpl in Hp; try tauto.
-            simpl in H4. subst l; simpl in Hl. tauto.
+            simpl in *. subst l; simpl in Hl. tauto.
           - iAlways. iExists p''; iSplit; auto. destruct (Addr_le_dec b' e').
             + rewrite (isWithin_region_addrs_decomposition b' e' b e); try solve_addr.
               rewrite !big_sepL_app. iDestruct "A" as "[A1 [A2 A3]]".
-              iApply (big_sepL_impl with "A2"); auto. iAlways; iIntros (k y Hy) "[#Y [% %]]".
+              iApply (big_sepL_impl with "A2"); auto. iAlways; iIntros (k y Hy) "[#Y %]".
               repeat iSplitR; auto.
-              * iApply (region_state_future with "Hfuture"); eauto.
-              * iApply (region_std_future with "Hfuture"); eauto.
+              iApply (region_state_future with "Hfuture"); eauto.             
             + rewrite (region_addrs_empty b' e'); auto. solve_addr. }
         destruct p'; auto.
       - destruct Hp' as [Hp1 [Hp2 Hp3] ].
         destruct p'; auto; try congruence. }
     case_eq (pwl p'); intros; auto.
     assert (pwl p = true) as HP by (destruct p, p'; simpl in Hp; inv Hp; simpl in *; auto; try congruence).
-    rewrite HP in H4; subst l. destruct l'; simpl in Hl; auto.
+    rewrite HP in H0; subst l. destruct l'; simpl in Hl; auto.
   Qed.
 
 End fundamental.
