theories/ftlr/Get.v
@@ -6,12 +6,13 @@ From cap_machine Require Import ftlr_base.
 From cap_machine.rules Require Export rules_Get.
 
 Section fundamental.
-  Context `{memG Σ, regG Σ, STSG Σ, logrel_na_invs Σ,
-            MonRef: MonRefG (leibnizO _) CapR_rtc Σ,
-            Heap: heapG Σ}.
+  Context {Σ:gFunctors} {memg:memG Σ} {regg:regG Σ}
+          {stsg : STSG Addr region_type Σ} {heapg : heapG Σ}
+          `{MonRef: MonRefG (leibnizO _) CapR_rtc Σ} {nainv: logrel_na_invs Σ}.
 
   Notation STS := (leibnizO (STS_states * STS_rels)).
-  Notation WORLD := (leibnizO (STS * STS)).
+  Notation STS_STD := (leibnizO (STS_std_states Addr region_type)).
+  Notation WORLD := (prodO STS_STD STS). 
   Implicit Types W : WORLD.
 
   Notation D := (WORLD -n> (leibnizO Word) -n> iProp Σ).
@@ -24,7 +25,7 @@ Section fundamental.
     is_Get ins dst r0 →
     ftlr_instr W r p p' g b e a w ins ρ.
   Proof.
-    intros Hinstr Hp Hsome i Hbae Hfp Hpwl Hregion Hstd [Hnotrevoked Hnotstatic] HO Hi.
+    intros Hinstr Hp Hsome i Hbae Hfp Hpwl Hregion [Hnotrevoked Hnotstatic] HO Hi.
     iIntros "#IH #Hinv #Hreg #Hinva Hmono #Hw Hsts Hown".
     iIntros "Hr Hstate Ha HPC Hmap".
     rewrite delete_insert_delete.
