theories/ftlr/Restrict.v
@@ -6,12 +6,13 @@ From cap_machine Require Import ftlr_base monotone interp_weakening.
 From cap_machine.rules Require Import rules_Restrict.
 
 Section fundamental.
-  Context `{memG Σ, regG Σ, STSG Σ, logrel_na_invs Σ,
-            MonRef: MonRefG (leibnizO _) CapR_rtc Σ,
-            Heap: heapG Σ}.
+  Context {Σ:gFunctors} {memg:memG Σ} {regg:regG Σ}
+          {stsg : STSG Addr region_type Σ} {heapg : heapG Σ}
+          `{MonRef: MonRefG (leibnizO _) CapR_rtc Σ} {nainv: logrel_na_invs Σ}.
 
   Notation STS := (leibnizO (STS_states * STS_rels)).
-  Notation WORLD := (leibnizO (STS * STS)). 
+  Notation STS_STD := (leibnizO (STS_std_states Addr region_type)).
+  Notation WORLD := (prodO STS_STD STS). 
   Implicit Types W : WORLD.
 
   Notation D := (WORLD -n> (leibnizO Word) -n> iProp Σ).
@@ -28,7 +29,7 @@ Section fundamental.
   Lemma PermPairFlows_interp_preserved W p p' l l' b e a :
     p <> E ->
     PermPairFlowsTo (p', l') (p, l) = true →
-    □ ▷ (∀ (a7 : leibnizO (STS * STS)) (a8 : Reg) (a9 : Perm) (a10 : Locality) 
+    □ ▷ (∀ (a7 : WORLD) (a8 : Reg) (a9 : Perm) (a10 : Locality) 
            (a11 a12 a13 : Addr),
             full_map a8
             -∗ (∀ r1 : RegName,
@@ -40,7 +41,7 @@ Section fundamental.
                        end)
             -∗ registers_mapsto (<[PC:=inr (a9, a10, a11, a12, a13)]> a8)
             -∗ region a7
-            -∗ sts_full_world sts_std a7
+            -∗ sts_full_world a7
             -∗ na_own logrel_nais ⊤
             -∗ ⌜a9 = RX ∨ a9 = RWX ∨ a9 = RWLX ∧ a10 = Local⌝
             → □ (∃ p'0 : Perm,
@@ -49,17 +50,16 @@ Section fundamental.
                        read_write_cond a14 p'0 interp
                        ∧ ⌜if pwl a9
                           then region_state_pwl a7 a14
-                          else region_state_nwl a7 a14 a10⌝
-                               ∧ ⌜region_std a7 a14⌝)) -∗ 
+                          else region_state_nwl a7 a14 a10⌝)) -∗ 
                 interp_conf a7) -∗
     (fixpoint interp1) W (inr (p, l, b, e, a)) -∗
     (fixpoint interp1) W (inr (p', l', b, e, a)).
   Proof.
     intros HpnotE Hp. iIntros "#IH HA".
     destruct (andb_true_eq _ _ ltac:(symmetry in Hp; exact Hp)).
-    simpl in H3, H4. iApply (interp_weakening with "IH HA"); eauto; try solve_addr.
-    - rewrite <- H3. auto.
-    - rewrite <- H4. auto.
+    simpl in H, H0. iApply (interp_weakening with "IH HA"); eauto; try solve_addr.
+    - rewrite <- H. auto.
+    - rewrite <- H0. auto.
   Qed.
 
   Lemma match_perm_with_E_rewrite:
@@ -76,7 +76,7 @@ Section fundamental.
         (g : Locality) (b e a : Addr) (w : Word) (ρ : region_type) (dst : RegName) (r0 : Z + RegName):
     ftlr_instr W r p p' g b e a w (Restrict dst r0) ρ.
   Proof.
-    intros Hp Hsome i Hbae Hfp Hpwl Hregion Hstd [Hnotrevoked Hnotstatic] HO Hi.
+    intros Hp Hsome i Hbae Hfp Hpwl Hregion [Hnotrevoked Hnotstatic] HO Hi.
     iIntros "#IH #Hinv #Hreg #Hinva Hmono #Hw Hsts Hown".
     iIntros "Hr Hstate Ha HPC Hmap".
     rewrite delete_insert_delete.
@@ -99,37 +99,37 @@ Section fundamental.
       assert (HPCr0: match r0 with inl _ => True | inr r0 => PC <> r0 end).
       { destruct r0; auto.
         intro; subst r0.
-        rewrite /= lookup_insert in H5. inv H5. }
+        rewrite /= lookup_insert in H1. inv H1. }
 
       destruct (reg_eq_dec PC dst).
       { subst dst. repeat rewrite insert_insert.
         repeat rewrite insert_insert in HPC.
         rewrite lookup_insert in HPC. inv HPC.
-        rewrite lookup_insert in H3. inv H3.
-        rewrite H8 in H6. iDestruct (region_close with "[$Hstate $Hr $Ha $Hmono]") as "Hr"; eauto.
+        rewrite lookup_insert in H. inv H.
+        rewrite H4 in H2. iDestruct (region_close with "[$Hstate $Hr $Ha $Hmono]") as "Hr"; eauto.
         { destruct ρ;auto;[|specialize (Hnotstatic g)];contradiction. }
         destruct (PermFlowsTo RX p'') eqn:Hpft.
         { assert (Hpg: p'' = RX ∨ p'' = RWX ∨ p'' = RWLX ∧ g'' = Local).
           { destruct p''; simpl in Hpft; eauto; try discriminate.
-            destruct (andb_true_eq _ _ ltac:(symmetry in H6; exact H6)).
-            simpl in H3, H7. destruct p0; simpl in H3; try discriminate.
+            destruct (andb_true_eq _ _ ltac:(symmetry in H2;exact H2)).
+            simpl in H2, H3. destruct p0; simpl in H2; try discriminate.
             destruct Hp as [Hp | [Hp | [Hp Hg] ] ]; try discriminate.
-            subst g0; destruct g''; simpl in H7; auto; discriminate. }
-          rewrite H8. iApply ("IH" $! _ r with "[%] [] [Hmap] [$Hr] [$Hsts] [$Hown]"); try iClear "IH"; eauto.
+            subst g0; destruct g''; simpl in H3; auto; discriminate. }
+          rewrite H4. iApply ("IH" $! _ r with "[%] [] [Hmap] [$Hr] [$Hsts] [$Hown]"); try iClear "IH"; eauto.
           iAlways. iExists p'. iSplitR.
-          - destruct (andb_true_eq _ _ ltac:(symmetry in H6; exact H6)).
-            iPureIntro. eapply PermFlows_trans with p0; auto. symmetry; exact H3.
+          - destruct (andb_true_eq _ _ ltac:(symmetry in H2; exact H2)).
+            iPureIntro. eapply PermFlows_trans with p0; auto. symmetry; exact H.
           - iApply (big_sepL_mono with "Hinv"); simpl; intros.
-            iIntros "[H [% %]]". iSplitL; auto.
-            iPureIntro; split; auto.
-            destruct (andb_true_eq _ _ ltac:(symmetry in H6; exact H6)); simpl in H10, H11.
+            iIntros "[H %]". iSplitL; auto.
+            iPureIntro. 
+            destruct (andb_true_eq _ _ ltac:(symmetry in H2; exact H2)); simpl in *.
             destruct (locality_eq_dec g'' g0).
-            * subst g0. destruct Hp as [Hp | [ Hp | [Hp Hl] ] ]; destruct Hpg as [Hp' | [ Hp' | [Hp' Hg' ] ] ]; subst; simpl in H10, H7; simpl; try congruence; auto.
-            * destruct g''; destruct g0; simpl in H11; try congruence.
-              destruct Hp as [Hp | [ Hp | [Hp Hl] ] ]; destruct Hpg as [Hp' | [ Hp' | [Hp' Hg' ] ] ]; subst; simpl in H10, H7; simpl; try congruence; auto. }
+            * subst g0. destruct Hp as [Hp | [ Hp | [Hp Hl] ] ]; destruct Hpg as [Hp' | [ Hp' | [Hp' Hg' ] ] ]; subst; simpl in *; simpl; try congruence; auto.
+            * destruct g''; destruct g0; simpl in *; try congruence.
+              destruct Hp as [Hp | [ Hp | [Hp Hl] ] ]; destruct Hpg as [Hp' | [ Hp' | [Hp' Hg' ] ] ]; subst; simpl in *; simpl; try congruence; auto. }
         { iApply (wp_bind (fill [SeqCtx])).
           iDestruct ((big_sepM_delete _ _ PC) with "Hmap") as "[HPC Hmap]"; [apply lookup_insert|].
-          rewrite H8.
+         rewrite H4.
           iApply (wp_notCorrectPC with "HPC"); [eapply not_isCorrectPC_perm; destruct p''; simpl in Hpft; eauto; discriminate|].
           iNext. iIntros "HPC /=".
           iApply wp_pure_step_later; auto.
@@ -138,7 +138,7 @@ Section fundamental.
 
       rewrite lookup_insert_ne in HPC; auto.
       rewrite lookup_insert in HPC. inv HPC.
-      rewrite lookup_insert_ne in H3; auto.
+      rewrite lookup_insert_ne in H; auto.
       iDestruct (region_close with "[$Hstate $Hr $Ha $Hmono]") as "Hr"; eauto.
       { destruct ρ;auto;[|specialize (Hnotstatic g)];contradiction. }
       iApply ("IH" $! _ (<[dst:=_]> _) with "[%] [] [Hmap] [$Hr] [$Hsts] [$Hown]"); eauto.
@@ -148,7 +148,7 @@ Section fundamental.
         + subst ri. rewrite lookup_insert.
           destruct (decodePermPair n) as (p1 & g1).
           iDestruct ("Hreg" $! dst Hri) as "Hdst".
-          rewrite H3. iApply PermPairFlows_interp_preserved; eauto.
+          rewrite H. iApply PermPairFlows_interp_preserved; eauto.
         + repeat rewrite lookup_insert_ne; auto.
           iApply "Hreg"; auto. }
   Qed.
