theories/monotone.v
@@ -5,122 +5,82 @@ From iris.base_logic Require Export invariants na_invariants saved_prop.
 Import uPred.
 
 Section monotone.
-  Context `{memG Σ, regG Σ, STSG Σ, logrel_na_invs Σ,
-            MonRef: MonRefG (leibnizO _) CapR_rtc Σ,
-            Heap: heapG Σ}.
+  Context {Σ:gFunctors} {memg:memG Σ} {regg:regG Σ}
+          {stsg : STSG Addr region_type Σ} {heapg : heapG Σ}
+          `{MonRef: MonRefG (leibnizO _) CapR_rtc Σ} {nainv: logrel_na_invs Σ}.
 
   Notation STS := (leibnizO (STS_states * STS_rels)).
-  Notation WORLD := (leibnizO (STS * STS)). 
+  Notation STS_STD := (leibnizO (STS_std_states Addr region_type)).
+  Notation WORLD := (prodO STS_STD STS). 
   Implicit Types W : WORLD.
   
   Lemma region_state_nwl_monotone W W' a l :
-    rel_is_std_i W (countable.encode a) →
     related_sts_pub_world W W' →
     region_state_nwl W a l -> region_state_nwl W' a l.
   Proof.
-    rewrite /region_state_nwl /std_sta /std_rel.
-    intros Hsome Hrelated Hstate.
+    rewrite /region_state_nwl /std. 
+    intros Hrelated Hstate.
     destruct l.
-    - apply (related_sts_rel_std W W') in Hsome as Hsome'; 
-        [|destruct Hrelated as [Hrelated1 Hrelated2]; split; apply related_sts_pub_priv; auto].
-      destruct Hrelated as [ [Hdom_sta [Hdom_rel Hrelated] ] _]. simpl in *.
-      specialize (Hrelated (countable.encode a) _ _ _ _ Hsome Hsome') as (_ & _ & Hrelated).
-      assert (is_Some (W'.1.1 !! countable.encode a)) as [y Hy].
+    - destruct Hrelated as [ [Hdom_sta Hrelated ] _]. simpl in *.
+      assert (is_Some (W'.1 !! a)) as [y Hy].
       { apply elem_of_gmap_dom. apply elem_of_subseteq in Hdom_sta. apply Hdom_sta. apply elem_of_gmap_dom;eauto. }
-      specialize (Hrelated (countable.encode Permanent) y Hstate Hy).
-      destruct (decide (y = countable.encode Permanent)); subst; auto.
-      apply std_rel_pub_rtc_Permanent in Hrelated; auto. contradiction. 
-    - apply (related_sts_rel_std W W') in Hsome as Hsome';
-        [|destruct Hrelated as [Hrelated1 Hrelated2]; split; apply related_sts_pub_priv; auto].
-      destruct Hrelated as [ [Hdom_sta [Hdom_rel Hrelated] ] _]. simpl in *.
-      specialize (Hrelated (countable.encode a) _ _ _ _ Hsome Hsome') as (_ & _ & Hrelated).
-      assert (is_Some (W'.1.1 !! countable.encode a)) as [y Hy].
+      specialize (Hrelated a Permanent y Hstate Hy).
+      apply std_rel_pub_rtc_Permanent in Hrelated; subst; auto. 
+    - destruct Hrelated as [ [Hdom_sta Hrelated] _]. simpl in *.
+      assert (is_Some (W'.1 !! a)) as [y Hy].
       { apply elem_of_gmap_dom. apply elem_of_subseteq in Hdom_sta. apply Hdom_sta. apply elem_of_gmap_dom.
         destruct Hstate; eauto. }
       destruct Hstate as [HTemp | HPerm].
       + left. 
-        specialize (Hrelated (countable.encode Temporary) y HTemp Hy).
-        destruct (decide (y = countable.encode Temporary)); subst; auto.
-        apply std_rel_pub_rtc_Temporary in Hrelated; auto. contradiction. 
+        specialize (Hrelated _ Temporary y HTemp Hy).
+        apply std_rel_pub_rtc_Temporary in Hrelated; subst;auto. 
       + right.
-        specialize (Hrelated (countable.encode Permanent) y HPerm Hy).
-        destruct (decide (y = countable.encode Permanent)); subst; auto.
-        apply std_rel_pub_rtc_Permanent in Hrelated; auto. contradiction. 
+        specialize (Hrelated _ Permanent y HPerm Hy).
+        apply std_rel_pub_rtc_Permanent in Hrelated; subst; auto. 
   Qed.
 
   Lemma region_state_nwl_monotone_nl W W' a :
-    rel_is_std_i W (countable.encode a) →
     related_sts_priv_world W W' →
     region_state_nwl W a Global -> region_state_nwl W' a Global.
   Proof.
-    rewrite /region_state_nwl /std_sta /std_rel.
-    intros Hsome Hrelated Hstate.
-    apply (related_sts_rel_std W W') in Hsome as Hsome'; auto. 
-    
-    destruct Hrelated as [ [Hdom_sta [Hdom_rel Hrelated] ] _].
-    specialize (Hrelated (countable.encode a) _ _ _ _ Hsome Hsome') as (_ & _ & Hrelated).
-    assert (is_Some (W'.1.1 !! countable.encode a)) as [y Hy].
+    rewrite /region_state_nwl /std.
+    intros Hrelated Hstate.
+    destruct Hrelated as [ [Hdom_sta Hrelated ] _].
+    assert (is_Some (W'.1 !! a)) as [y Hy].
     { apply elem_of_gmap_dom. apply elem_of_subseteq in Hdom_sta. apply Hdom_sta. apply elem_of_gmap_dom;eauto. }
-    specialize (Hrelated (countable.encode Permanent) y Hstate Hy).
-    destruct (decide (y = countable.encode Permanent)); subst; auto.
-    apply std_rel_rtc_Permanent in Hrelated; auto. contradiction. 
+    specialize (Hrelated _ Permanent y Hstate Hy).
+    apply std_rel_rtc_Permanent in Hrelated; subst; auto. 
   Qed.
 
   Lemma region_state_pwl_monotone W W' a :
-    rel_is_std_i W (countable.encode a) →
     related_sts_pub_world W W' →
     region_state_pwl W a -> region_state_pwl W' a.
   Proof.
-    rewrite /region_state_pwl /std_sta /std_rel.
-    intros Hsome Hrelated Hstate.
-    apply (related_sts_rel_std W W') in Hsome as Hsome'; 
-      [|destruct Hrelated as [Hrelated1 Hrelated2]; split; apply related_sts_pub_priv; auto].
-    destruct Hrelated as [ [Hdom_sta [Hdom_rel Hrelated] ] _]. simpl in *.
-    specialize (Hrelated (countable.encode a) _ _ _ _ Hsome Hsome') as (_ & _ & Hrelated).
-    assert (is_Some (W'.1.1 !! countable.encode a)) as [y Hy].
+    rewrite /region_state_pwl /std.
+    intros Hrelated Hstate.
+    destruct Hrelated as [ [Hdom_sta Hrelated ] _]. simpl in *.
+    assert (is_Some (W'.1 !! a)) as [y Hy].
     { apply elem_of_gmap_dom. apply elem_of_subseteq in Hdom_sta. apply Hdom_sta. apply elem_of_gmap_dom;eauto. }
-    specialize (Hrelated (countable.encode Temporary) y Hstate Hy).
-    destruct (decide (y = countable.encode Temporary)); subst; auto.
-    apply std_rel_pub_rtc_Temporary in Hrelated; auto. contradiction. 
+    specialize (Hrelated _ Temporary y Hstate Hy).
+    apply std_rel_pub_rtc_Temporary in Hrelated; subst; auto. 
   Qed.
 
   Lemma region_state_Revoked_monotone (W W' : WORLD) (a : Addr) :
-    rel_is_std_i W (countable.encode a) →
     related_sts_pub_world W W' →
-    (std_sta W) !! (countable.encode a) = Some (countable.encode Revoked) ->
-    (std_sta W') !! (countable.encode a) = Some (countable.encode Revoked) ∨
-    (std_sta W') !! (countable.encode a) = Some (countable.encode Temporary).
+    (std W) !! a = Some Revoked ->
+    (std W') !! a = Some Revoked ∨
+    (std W') !! a = Some Temporary.
   Proof.
-    rewrite /region_state_pwl /std_sta /std_rel.
-    intros Hsome Hrelated Hstate.
-    apply (related_sts_rel_std W W') in Hsome as Hsome'; 
-      [|destruct Hrelated as [Hrelated1 Hrelated2]; split; apply related_sts_pub_priv; auto].
-    destruct Hrelated as [ [Hdom_sta [Hdom_rel Hrelated] ] _]. simpl in *.
-    specialize (Hrelated (countable.encode a) _ _ _ _ Hsome Hsome') as (_ & _ & Hrelated).
-    assert (is_Some (W'.1.1 !! countable.encode a)) as [y Hy].
+    rewrite /region_state_pwl /std. 
+    intros Hrelated Hstate.
+    destruct Hrelated as [ [Hdom_sta Hrelated ] _]. simpl in *.
+    assert (is_Some (W'.1 !! a)) as [y Hy].
     { apply elem_of_gmap_dom. apply elem_of_subseteq in Hdom_sta. apply Hdom_sta. apply elem_of_gmap_dom;eauto. }
-    specialize (Hrelated (countable.encode Revoked) y Hstate Hy).
+    specialize (Hrelated _ Revoked y Hstate Hy).
     apply std_rel_pub_rtc_Revoked in Hrelated; auto.
     destruct Hrelated as [Htemp | Hrev]; subst; auto. 
   Qed.
-  
-  Lemma rel_is_std_i_monotone (W W' : WORLD) (a : Addr) :
-    related_sts_pub_world W W' →
-    rel_is_std_i W (countable.encode a) →
-    rel_is_std_i W' (countable.encode a).
-  Proof.
-    rewrite /rel_is_std_i.
-    intros [(Hdom_sta & Hdom_rel & Htransition) _] Hstd.
-    apply elem_of_subseteq in Hdom_rel.
-    assert ((countable.encode a) ∈ dom (gset positive) (std_rel W)) as Hin.
-    { apply elem_of_dom. eauto. }
-    specialize (Hdom_rel (countable.encode a) Hin).
-    apply elem_of_dom in Hdom_rel as [ [r1' r2'] Hr'].
-    apply elem_of_dom in Hin as [ [r1 r2] Hr].
-    specialize (Htransition (countable.encode a) r1 r2 r1' r2' Hr Hr') as (Heq1 & Heq2 & _). 
-    simplify_eq. rewrite Hstd in Hr. inversion Hr. subst. auto.
-  Qed. 
-    
+      
   Lemma interp_monotone W W' w :
     (⌜related_sts_pub_world W W'⌝ →
     interp W w -∗ interp W' w)%I. 
@@ -132,33 +92,29 @@ Section monotone.
     - iDestruct "Hw" as (p Hfl) "Hw".
       iExists _; iSplit;eauto.
       iApply (big_sepL_mono with "Hw").
-      iIntros (n y Hsome) "#[Hrw [Hst Hrel] ]". iFrame "#".
-      iDestruct "Hst" as %Hst; iDestruct "Hrel" as %Hrel. 
-      iPureIntro. split; [apply region_state_nwl_monotone with W|apply related_sts_rel_std with W]; auto.
-      apply related_sts_pub_priv_world; auto.
+      iIntros (n y Hsome) "#[Hrw Hrel]". iFrame "#".
+      iDestruct "Hrel" as %Hrel. 
+      iPureIntro. apply region_state_nwl_monotone with W;auto. 
     - iDestruct "Hw" as (p Hfl) "Hw".
       iExists _; iSplit;eauto.
       iApply (big_sepL_mono with "Hw").
-      iIntros (n y Hsome) "#[Hrw [Hst Hrel] ]". iFrame "#".
-      iDestruct "Hst" as %Hst; iDestruct "Hrel" as %Hrel. 
-      iPureIntro. split; [apply region_state_nwl_monotone with W|apply related_sts_rel_std with W]; auto.
-      apply related_sts_pub_priv_world; auto.
+      iIntros (n y Hsome) "#[Hrw Hrel]". iFrame "#".
+      iDestruct "Hrel" as %Hrel. 
+      iPureIntro. apply region_state_nwl_monotone with W;auto. 
     - destruct l; auto. 
       iDestruct "Hw" as (p Hfl) "Hw".
       iExists _; iSplit;eauto.
       iApply (big_sepL_mono with "Hw").
-      iIntros (n y Hsome) "#[Hrw [Hst Hrel] ]". iFrame "#".
-      iDestruct "Hst" as %Hst; iDestruct "Hrel" as %Hrel. 
-      iPureIntro. split; [apply region_state_pwl_monotone with W|apply related_sts_rel_std with W]; auto.
-      apply related_sts_pub_priv_world; auto. 
+      iIntros (n y Hsome) "#[Hrw Hrel]". iFrame "#".
+      iDestruct "Hrel" as %Hrel. 
+      iPureIntro. apply region_state_pwl_monotone with W;auto. 
     - iDestruct "Hw" as (p Hfl) "[Hbe Hexec]".
       iExists _. iSplitR;[eauto|].
       iSplit.
       { iApply (big_sepL_mono with "Hbe").
-        iIntros (n y Hsome) "#[Hrw [Hst Hrel] ]". iFrame "#".
-        iDestruct "Hst" as %Hst; iDestruct "Hrel" as %Hrel. 
-        iPureIntro. split; [apply region_state_nwl_monotone with W|apply related_sts_rel_std with W]; auto.
-        apply related_sts_pub_priv_world; auto. }
+        iIntros (n y Hsome) "#[Hrw Hrel ]". iFrame "#".
+        iDestruct "Hrel" as %Hrel. 
+        iPureIntro. apply region_state_nwl_monotone with W;auto. }
       iAlways.
       iIntros (a' r' W'' Hin).
       destruct l; simpl.
@@ -188,10 +144,9 @@ Section monotone.
       iExists p. iSplit;[auto|].
       iSplit.
       { iApply (big_sepL_mono with "Hbe").
-        iIntros (n y Hsome) "#[Hrw [Hst Hrel] ]". iFrame "#".
-        iDestruct "Hst" as %Hst; iDestruct "Hrel" as %Hrel. 
-        iPureIntro. split; [apply region_state_nwl_monotone with W|apply related_sts_rel_std with W]; auto.
-        apply related_sts_pub_priv_world; auto. }
+        iIntros (n y Hsome) "#[Hrw Hrel ]". iFrame "#".
+        iDestruct "Hrel" as %Hrel. 
+        iPureIntro. apply region_state_nwl_monotone with W;auto. }        
       iAlways. iIntros (a' r W'' Hin).
       destruct l; simpl.
       + iIntros (Hrelated').
@@ -213,10 +168,9 @@ Section monotone.
       iExists p. iSplit;[auto|].
       iSplit.
       { iApply (big_sepL_mono with "Hbe").
-        iIntros (n y Hsome) "#[Hrw [Hst Hrel] ]". iFrame "#".
-        iDestruct "Hst" as %Hst; iDestruct "Hrel" as %Hrel. 
-        iPureIntro. split; [apply region_state_pwl_monotone with W|apply related_sts_rel_std with W]; auto.
-        apply related_sts_pub_priv_world; auto. }
+        iIntros (n y Hsome) "#[Hrw Hrel ]". iFrame "#".
+        iDestruct "Hrel" as %Hrel. 
+        iPureIntro. apply region_state_pwl_monotone with W;auto. }        
       iAlways. iIntros (a' r W'' Hin).
       iIntros (Hrelated').
       iAssert (future_world Local W W'')%I as "Hrelated".
@@ -238,26 +192,26 @@ Section monotone.
     - iDestruct "Hw" as (p Hfl) "Hw".
       iExists _; iSplit;eauto.
       iApply (big_sepL_mono with "Hw").
-      iIntros (n y Hsome) "#[Hrw [Hst Hrel] ]". iFrame "#".
-      iDestruct "Hst" as %Hst; iDestruct "Hrel" as %Hrel. 
+      iIntros (n y Hsome) "#[Hrw Hrel ]". iFrame "#".
+      iDestruct "Hrel" as %Hrel. 
       iPureIntro. destruct l; try discriminate. 
-      split; [apply region_state_nwl_monotone_nl with W|apply related_sts_rel_std with W]; auto.
+      apply region_state_nwl_monotone_nl with W;auto. 
     - iDestruct "Hw" as (p Hfl) "Hw".
       iExists _; iSplit;eauto.
       iApply (big_sepL_mono with "Hw").
-      iIntros (n y Hsome) "#[Hrw [Hst Hrel] ]". iFrame "#".
-      iDestruct "Hst" as %Hst; iDestruct "Hrel" as %Hrel. 
+      iIntros (n y Hsome) "#[Hrw Hrel ]". iFrame "#".
+      iDestruct "Hrel" as %Hrel. 
       iPureIntro. destruct l; try discriminate. 
-      split; [apply region_state_nwl_monotone_nl with W|apply related_sts_rel_std with W]; auto.
+      apply region_state_nwl_monotone_nl with W;auto. 
     - destruct l; auto. discriminate. 
     - iDestruct "Hw" as (p Hfl) "[Hbe Hexec]".
       iExists _. iSplitR;[eauto|].
       iSplit.
       { iApply (big_sepL_mono with "Hbe").
-        iIntros (n y Hsome) "#[Hrw [Hst Hrel] ]". iFrame "#".
-        iDestruct "Hst" as %Hst; iDestruct "Hrel" as %Hrel. 
+        iIntros (n y Hsome) "#[Hrw Hrel]". iFrame "#".
+        iDestruct "Hrel" as %Hrel. 
         iPureIntro. destruct l; try discriminate.
-        split; [apply region_state_nwl_monotone_nl with W|apply related_sts_rel_std with W]; auto. }
+        apply region_state_nwl_monotone_nl with W;auto. }
       iAlways.
       iIntros (a' r' W'' Hin).
       destruct l; simpl; try discriminate.
@@ -277,10 +231,10 @@ Section monotone.
       iExists p. iSplit;[auto|].
       iSplit.
       { iApply (big_sepL_mono with "Hbe").
-        iIntros (n y Hsome) "#[Hrw [Hst Hrel] ]". iFrame "#".
-        iDestruct "Hst" as %Hst; iDestruct "Hrel" as %Hrel. 
+        iIntros (n y Hsome) "#[Hrw Hrel ]". iFrame "#".
+        iDestruct "Hrel" as %Hrel. 
         iPureIntro. destruct l; try discriminate. 
-        split; [apply region_state_nwl_monotone_nl with W|apply related_sts_rel_std with W]; auto. }
+        apply region_state_nwl_monotone_nl with W;auto. }
       iAlways. iIntros (a' r W'' Hin).
       destruct l; simpl; try discriminate.
       iIntros (Hrelated').
@@ -319,14 +273,14 @@ Section monotone.
 
 
 Global Instance interp_ne n :
-  Proper (dist n ==> dist n) (λ Wv : prodO (leibnizO (STS * STS)) (leibnizO Word), (interp Wv.1) Wv.2).
+  Proper (dist n ==> dist n) (λ Wv : WORLD * (leibnizO Word), (interp Wv.1) Wv.2).
 Proof.
   solve_proper.
 Qed.
 
 (*The general monotonicity statement that interp gives you when writing a word into a pointer (p0, l, a2, a1, a0) ; simply a bundling of all individual monotonicity statements*)
 Lemma interp_monotone_generalW (W : WORLD)  (ρ : region_type) (p p0 p1 : Perm) (l g : Locality)(b e a a2 a1 a0 : Addr):
-  std_sta W !! countable.encode a0 = Some (countable.encode ρ) →
+  std W !! a0 = Some ρ →
   withinBounds (p0, l, a2, a1, a0) = true →
   PermFlows p0 p1 →
   (negb (isLocal g) || match p0 with
@@ -334,7 +288,7 @@ Lemma interp_monotone_generalW (W : WORLD)  (ρ : region_type) (p p0 p1 : Perm) 
                        | _ => false
                        end = true)→
   ((fixpoint interp1) W) (inr (p0, l, a2, a1, a0)) -∗
-  monotonicity_guarantees_region ρ  (inr (p, g, b, e, a)) p1  (λne Wv : prodO (leibnizO (STS * STS)) (leibnizO Word), (interp Wv.1) Wv.2).
+  monotonicity_guarantees_region ρ  (inr (p, g, b, e, a)) p1  (λne Wv : WORLD * (leibnizO Word), (interp Wv.1) Wv.2).
 Proof.
   unfold monotonicity_guarantees_region.
   iIntros (Hstd Hwb Hfl' Hconds) "#Hvdst".
@@ -353,20 +307,18 @@ Proof.
     + by iApply interp_monotone_nl.
     + (*Trick here: value relation leads to a contradiction if p0 is WL, since then its region cannot be permanent*)
       iDestruct ( writeLocalAllowed_valid_cap_implies with "Hvdst" ) as "%"; eauto.
-      destruct H3. rewrite Hstd in H4. inversion H4.
-      apply (f_equal (countable.decode (A:=region_type))) in H6.
-      do 2 rewrite countable.decode_encode in H6. by inversion H6.
-         - auto.
-         - auto. 
+      rewrite Hstd in H. inversion H.
+  - auto.
+  - auto. 
 Qed.
 
 (* Analogous, but now we have the general monotonicity statement in case an integer z is written *)
 Lemma interp_monotone_generalZ (W : WORLD)  (ρ : region_type) (p0 p1 : Perm) (l : Locality)(a2 a1 a0 : Addr) z:
-  std_sta W !! countable.encode a0 = Some (countable.encode ρ) →
+  std W !! a0 = Some ρ →
   withinBounds (p0, l, a2, a1, a0) = true →
   PermFlows p0 p1 →
   ((fixpoint interp1) W) (inr (p0, l, a2, a1, a0)) -∗
-  monotonicity_guarantees_region ρ  (inl z) p1  (λne Wv : prodO (leibnizO (STS * STS)) (leibnizO Word), (interp Wv.1) Wv.2).
+  monotonicity_guarantees_region ρ  (inl z) p1  (λne Wv : WORLD * (leibnizO Word), (interp Wv.1) Wv.2).
 Proof.
   unfold monotonicity_guarantees_region.
   iIntros (Hstd Hwb Hfl') "#Hvdst".
